tuned formatting

thys/Transitive-Closure/Transitive_Closure_List_Impl.thy
@@ -5,134 +5,145 @@
     License:     LGPL
 *)
 
-header {* Closure computation on lists *}
+header {* Closure Computation using Lists *}
 
 theory Transitive_Closure_List_Impl
 imports Transitive_Closure_Impl
 begin
 
-text {*
-\label{closure list}
-We provide two algorithms for the computation of the reflexive transitive
-closure which internally work on lists.  The first one (@{term
-rtrancl_list_impl}) computes the closure on demand for a given set of initial
-states.  The second one (@{term memo_list_rtrancl}) precomputes the closure for
-each individual state, stores these results, and then only does a look-up.
+text \<open>
+  We provide two algorithms for the computation of the reflexive transitive closure which internally
+  work on lists. The first one (@{term rtrancl_list_impl}) computes the closure on demand for a
+  given set of initial states. The second one (@{term memo_list_rtrancl}) precomputes the closure
+  for each individual state, stores the result, and then only does a look-up.
+  
+  For the transitive closure there are the corresponding algorithms @{term trancl_list_impl} and
+  @{term memo_list_trancl}.
+\<close>
 
-For the transitive closure there are the corresponding algorithms @{term
-trancl_list_impl} and @{term memo_list_trancl}
-*}
+subsection \<open>Computing Closures from Sets On-The-Fly\<close>
 
-subsection {* Computing closures from sets on-the-fly *} 
+text \<open>
+  The algorithms are based on the generic algorithms @{const rtrancl_impl} and @{const trancl_impl}
+  instantiated by list operations. Here, after computing the successors in a straightforward way,
+  we use @{const remdups} to not have duplicates in the results. Moreover, also in the union
+  operation we filter to those elements that have not yet been seen. The use of @{const filter} in
+  the union operation is preferred over @{const remdups} since by construction the latter set will
+  not contain duplicates.
+\<close>
 
-text {*
-The algorithms are based on the generic algorithms @{const rtrancl_impl} and
-@{const trancl_impl} instantiated by list operations. Here, after computing the
-successors in a straightforwards way, we use @{const remdups} to not have
-duplicates in the results.  Moreover, also in the union operation we filter to
-those elements that have not yet been seen.  The use of @{const filter} in the
-union operation is preferred over @{const remdups} since by construction the
-latter set will not contain duplicates.
-*} 
+definition rtrancl_list_impl :: "('a \<times> 'a) list \<Rightarrow> 'a list \<Rightarrow> 'a list"
+where
+  "rtrancl_list_impl = rtrancl_impl
+    (\<lambda> r as. remdups (map snd (filter (\<lambda> (a, b). a \<in> set as) r)))
+    (\<lambda> xs ys. (filter (\<lambda> x. x \<notin> set ys) xs) @ ys)
+    (\<lambda> x xs. x \<in> set xs)
+    []"
 
-definition rtrancl_list_impl :: "('a \<times> 'a)list \<Rightarrow> 'a list \<Rightarrow> 'a list"
-  where "rtrancl_list_impl \<equiv> rtrancl_impl (\<lambda> r as. remdups (map snd (filter (\<lambda> (a,b). a \<in> set as) r))) (\<lambda> xs ys. (filter (\<lambda> x. x \<notin> set ys) xs) @ ys)  (\<lambda> x xs. x \<in> set xs) []"
+definition trancl_list_impl :: "('a \<times> 'a) list \<Rightarrow> 'a list \<Rightarrow> 'a list"
+where
+  "trancl_list_impl = trancl_impl
+    (\<lambda> r as. remdups (map snd (filter (\<lambda> (a, b). a \<in> set as) r)))
+    (\<lambda> xs ys. (filter (\<lambda> x. x \<notin> set ys) xs) @ ys)
+    (\<lambda> x xs. x \<in> set xs)
+    []"
 
-definition trancl_list_impl :: "('a \<times> 'a)list \<Rightarrow> 'a list \<Rightarrow> 'a list"
-  where "trancl_list_impl \<equiv> trancl_impl (\<lambda> r as. remdups (map snd (filter (\<lambda> (a,b). a \<in> set as) r))) (\<lambda> xs ys. (filter (\<lambda> x. x \<notin> set ys) xs) @ ys)  (\<lambda> x xs. x \<in> set xs) []"
-
-lemma rtrancl_list_impl: "set (rtrancl_list_impl r as) = {b. \<exists> a \<in> set as. (a,b) \<in> (set r)^*}"
+lemma rtrancl_list_impl:
+  "set (rtrancl_list_impl r as) = {b. \<exists> a \<in> set as. (a, b) \<in> (set r)\<^sup>*}"
   unfolding rtrancl_list_impl_def
   by (rule set_access_gen.rtrancl_impl, unfold_locales, force+)
 
-lemma trancl_list_impl: "set (trancl_list_impl r as) = {b. \<exists> a \<in> set as. (a,b) \<in> (set r)^+}"
+lemma trancl_list_impl:
+  "set (trancl_list_impl r as) = {b. \<exists> a \<in> set as. (a, b) \<in> (set r)\<^sup>+}"
   unfolding trancl_list_impl_def
   by (rule set_access_gen.trancl_impl, unfold_locales, force+)
 
 
-subsection {* Precomputing closures for single states *}
+subsection \<open>Precomputing Closures for Single States\<close>
 
-text {* Storing all relevant entries is done by mapping all left-hand sides of the relation
-  to their closure. To avoid redundant entries, @{const remdups} is used.
-*}
+text \<open>
+  Storing all relevant entries is done by mapping all left-hand sides of the relation to their
+  closure. To avoid redundant entries, @{const remdups} is used.
+\<close>
 
-definition memo_list_rtrancl :: "('a \<times> 'a) list \<Rightarrow> ('a \<Rightarrow> 'a list)" where
-  "memo_list_rtrancl r \<equiv>
-    let
+definition memo_list_rtrancl :: "('a \<times> 'a) list \<Rightarrow> ('a \<Rightarrow> 'a list)"
+where
+  "memo_list_rtrancl r =
+    (let
       tr = rtrancl_list_impl r;
-      rm = map (\<lambda>a. (a, tr [a])) ((remdups o map fst) r)
+      rm = map (\<lambda>a. (a, tr [a])) ((remdups \<circ> map fst) r)
     in
       (\<lambda>a. case map_of rm a of
         None \<Rightarrow> [a]
-      | Some as \<Rightarrow> as)"
+      | Some as \<Rightarrow> as))"
 
 lemma memo_list_rtrancl:
-  "set (memo_list_rtrancl r a) = {b. (a,b) \<in> (set r)^*}" (is "?l = ?r")
+  "set (memo_list_rtrancl r a) = {b. (a, b) \<in> (set r)\<^sup>*}" (is "?l = ?r")
 proof -
-  let ?rm = "map (\<lambda> a. (a, rtrancl_list_impl r [a])) ((remdups o map fst) r)"
+  let ?rm = "map (\<lambda> a. (a, rtrancl_list_impl r [a])) ((remdups \<circ> map fst) r)"
   show ?thesis
   proof (cases "map_of ?rm a")
     case None
     have one: "?l = {a}"
       unfolding memo_list_rtrancl_def Let_def None
       by auto
-    from None[unfolded map_of_eq_None_iff]
+    from None [unfolded map_of_eq_None_iff]
     have a: "a \<notin> fst ` set r" by force
     {
       fix b
       assume "b \<in> ?r"
-      from this[unfolded rtrancl_power relpow_fun_conv] obtain n f where 
+      from this [unfolded rtrancl_power relpow_fun_conv] obtain n f where 
         ab: "f 0 = a \<and> f n = b" and steps: "\<And> i. i < n \<Longrightarrow> (f i, f (Suc i)) \<in> set r" by auto
-      from ab steps[of 0] a have "a = b" 
+      from ab steps [of 0] a have "a = b" 
         by (cases n, force+)
     }
-    hence "?r = {a}" by auto
-    thus ?thesis unfolding one by simp
+    then have "?r = {a}" by auto
+    then show ?thesis unfolding one by simp
   next
     case (Some as) 
-    have as: "set as = {b. (a,b) \<in> (set r)^*}"
-      using map_of_is_SomeD[OF Some]
-        rtrancl_list_impl[of r "[a]"] by force
-    thus ?thesis unfolding memo_list_rtrancl_def Let_def Some by simp
+    have as: "set as = {b. (a, b) \<in> (set r)^*}"
+      using map_of_is_SomeD [OF Some]
+        rtrancl_list_impl [of r "[a]"] by force
+    then show ?thesis unfolding memo_list_rtrancl_def Let_def Some by simp
   qed
 qed
 
-
-definition memo_list_trancl :: "('a \<times> 'a) list \<Rightarrow> ('a \<Rightarrow> 'a list)" where
-  "memo_list_trancl r \<equiv>
-    let
+definition memo_list_trancl :: "('a \<times> 'a) list \<Rightarrow> ('a \<Rightarrow> 'a list)"
+where
+  "memo_list_trancl r =
+    (let
       tr = trancl_list_impl r;
-      rm = map (\<lambda>a. (a, tr [a])) ((remdups o map fst) r)
+      rm = map (\<lambda>a. (a, tr [a])) ((remdups \<circ> map fst) r)
     in
       (\<lambda>a. case map_of rm a of
         None \<Rightarrow> []
-      | Some as \<Rightarrow> as)"
+      | Some as \<Rightarrow> as))"
 
 lemma memo_list_trancl:
-  "set (memo_list_trancl r a) = {b. (a,b) \<in> (set r)^+}" (is "?l = ?r")
+  "set (memo_list_trancl r a) = {b. (a, b) \<in> (set r)\<^sup>+}" (is "?l = ?r")
 proof -
-  let ?rm = "map (\<lambda> a. (a, trancl_list_impl r [a])) ((remdups o map fst) r)"
+  let ?rm = "map (\<lambda> a. (a, trancl_list_impl r [a])) ((remdups \<circ> map fst) r)"
   show ?thesis
   proof (cases "map_of ?rm a")
     case None
     have one: "?l = {}"
       unfolding memo_list_trancl_def Let_def None
       by auto
-    from None[unfolded map_of_eq_None_iff]
+    from None [unfolded map_of_eq_None_iff]
       have a: "a \<notin> fst ` set r" by force
     {
       fix b
       assume "b \<in> ?r"
-      from this[unfolded trancl_unfold_left] a have False by force
+      from this [unfolded trancl_unfold_left] a have False by force
     }
-    hence "?r = {}" by auto
-    thus ?thesis unfolding one by simp
+    then have "?r = {}" by auto
+    then show ?thesis unfolding one by simp
   next
     case (Some as) 
-    have as: "set as = {b. (a,b) \<in> (set r)^+}"
-      using map_of_is_SomeD[OF Some]
+    have as: "set as = {b. (a, b) \<in> (set r)\<^sup>+}"
+      using map_of_is_SomeD [OF Some]
         trancl_list_impl[of r "[a]"] by force
-    thus ?thesis unfolding memo_list_trancl_def Let_def Some by simp
+    then show ?thesis unfolding memo_list_trancl_def Let_def Some by simp
   qed
 qed
 
